devel/Iron/Language/SystemF2Effect/Type/Lower.v
@@ -7,22 +7,20 @@ Require Import Iron.Language.SystemF2Effect.Type.Lift.
 (* Lowering of indices in types. *)
 Fixpoint lowerTT (d: nat) (tt: ty) : option ty 
  := match tt with
-    |  TCon _      => Some tt
-    |  TCap _      => Some tt
-
     |  TVar ix
     => match nat_compare ix d with
-       | Eq => None
-       | Gt => Some (TVar (ix - 1))
-       | _  => Some (TVar  ix)
+       | Eq                  => None
+       | Gt                  => Some (TVar (ix - 1))
+       | _                   => Some (TVar  ix)
        end
 
     |  TForall k t 
     => match lowerTT (S d) t with
-        | Some t2 => Some (TForall k t2)
-        | _       => None
+        | Some t2            => Some (TForall k t2)
+        | _                  => None
        end
 
+  
     |  TApp t1 t2
     => match lowerTT d t1, lowerTT d t2 with
         | Some t1', Some t2' => Some (TApp t1' t2')
@@ -36,69 +34,45 @@ Fixpoint lowerTT (d: nat) (tt: ty) : option ty
        end
 
     |  TBot k                => Some (TBot k)
+
+    |  TCon0 tc              => Some (TCon0 tc)
+
+    |  TCon1 tc t1
+    => match lowerTT d t1 with
+       | Some t1'            => Some (TCon1 tc t1')
+       | _                   => None
+       end
+
+    |  TCon2 tc t1 t2
+    => match lowerTT d t1, lowerTT d t2 with
+       | Some t1', Some t2'  => Some (TCon2 tc t1' t2')
+       | _, _                => None
+       end
+
+    |  TCap _                => Some tt
     end.
 
 
-(* Cleanup the Coqage here. 
-   How to we match on an 'if' scrutinee to remove the need for explicit
-   remembers?
-*)
 Lemma lowerTT_liftTT_some
  : forall t d d'
  , lowerTT d (liftTT 1 (1 + d + d') (liftTT 1 d t)) 
  = Some (liftTT 1 (d + d') t).
 Proof.
+ intros. gen d.
+ induction t; intros;
+  try burn;
+  try (solve [ simpl; split_match
+             ; repeat (rewritess; norm; auto)]).
+
 (* Keep this opaque so simpl doesn't unfold it *)
 Opaque le_gt_dec.
- intros. gen d.
- induction t; intros; burn.
-
  Case "TVar".
   simpl in *.
   lift_cases; simpl;
   lift_cases; simpl; 
   lift_cases; repeat (simpl; nnat); burn; try omega.
-
- Case "TForall".
-  simpl.
-  remember (lowerTT (S d) (liftTT 1 (S (S (d + d'))) (liftTT 1 (S d) t))) as X.
-  destruct X;
-  erewrite IHt in HeqX;
-   inverts HeqX; trivial.
-
- Case "TApp".
-  simpl.
-  remember (lowerTT d (liftTT 1 (S (d + d')) (liftTT 1 d t1))) as X.
-  destruct X;
-  erewrite IHt1 in HeqX.
-
-  remember (lowerTT d (liftTT 1 (S (d + d')) (liftTT 1 d t2))) as Y;
-  destruct Y.
-  erewrite IHt2 in HeqY; 
-   inverts HeqX; inverts HeqY; trivial.
-
-  inverts HeqX.
-  erewrite IHt2 in HeqY; nope.
-
-  nope.
-
- Case "TSum".
-  simpl.
-  remember (lowerTT d (liftTT 1 (S (d + d')) (liftTT 1 d t1))) as X.
-  destruct X;
-  erewrite IHt1 in HeqX.
-
-  remember (lowerTT d (liftTT 1 (S (d + d')) (liftTT 1 d t2))) as Y;
-  destruct Y.
-  erewrite IHt2 in HeqY; 
-   inverts HeqX; inverts HeqY; trivial.
-
-  inverts HeqX.
-  erewrite IHt2 in HeqY; nope.
-
-  nope.
 Transparent le_gt_dec.  
-Qed. 
+Qed.
 
 
 Lemma lowerTT_some_liftTT
@@ -108,48 +82,34 @@ Lemma lowerTT_some_liftTT
 Proof.
  intros. gen d t2.
  induction t1; intros;
-  try solve [inverts H; burn].
+  try burn;
+  try (solve [ norm; split_match
+             ; burn; try nope
+             ; repeat norm; f_equal; repeat norm; nope]).
 
  Case "TVar".
   simpl in *.
-  remember (nat_compare n d) as X.
-  destruct X; burn.
-  symmetry in HeqX. apply nat_compare_lt in HeqX.
-  inverts H. simpl. lift_cases; burn; omega.
-
-  symmetry in HeqX. apply nat_compare_gt in HeqX.
-  inverts H. simpl. lift_cases; burn.
-   destruct n; burn.
-   omega.
-
- Case "TForall".
-  simpl in *.
-  remember (lowerTT (S d) t1) as X.
-  destruct X.
-   inverts H.
-   simpl. f_equal. eauto.
-   false.
-
- Case "TApp".
-  simpl in *.
-  remember (lowerTT d t1_1) as X. destruct X; nope.
-  remember (lowerTT d t1_2) as X. destruct X; nope.
-  inverts H; burn. 
-   simpl.
-   rewrite IHt1_1; burn.
-   rewrite IHt1_2; burn.
-
- Case "TSum".
-  simpl in *.
-  remember (lowerTT d t1_1) as X. destruct X; nope.
-  remember (lowerTT d t1_2) as X. destruct X; nope.
-  inverts H; burn.
-   simpl.
-   rewrite IHt1_1; burn.
-   rewrite IHt1_2; burn.
+  split_match; burn.
+   norm. simpl. lift_cases; burn; omega.
+   norm. simpl. lift_cases; burn.
+    destruct n; burn. omega.
 Qed.
 Hint Resolve lowerTT_some_liftTT.
 Hint Rewrite lowerTT_some_liftTT.
+
+
+Lemma lowerTT_liftTT_succ
+ : forall d t1 t2
+ ,  lowerTT 0 t1                    = Some t2
+ -> lowerTT 0 (liftTT 1 (1 + d) t1) = Some (liftTT 1 d t2).
+Proof.
+ intros.
+ eapply lowerTT_some_liftTT in H.
+ symmetry in H. subst.
+ eapply lowerTT_liftTT_some.
+Qed.
+Hint Resolve lowerTT_liftTT_succ.
+Hint Rewrite lowerTT_liftTT_succ.
 
 
 Lemma lowerTT_liftTT
@@ -160,11 +120,7 @@ Proof.
  lift_burn t.
 
  Case "TVar".
-  simpl. lift_cases; simpl.
-  lift_cases; try omega.
-   repeat norm.
-
-  lift_cases; try omega. auto.
+  simpl; lift_cases; simpl; lift_cases; try omega; repeat norm.
 Qed.
 Hint Resolve lowerTT_liftTT.
 Hint Rewrite lowerTT_liftTT.
@@ -179,13 +135,10 @@ Proof.
  lift_burn t.
 
  Case "TVar".
-  simpl. 
-  lift_cases;
-   unfold liftTT;
-   lift_cases;
-    simpl; lift_cases; burn; omega.
+  simpl; 
+   lift_cases; unfold liftTT;
+   lift_cases; simpl; lift_cases; burn; omega.
 Qed.  
 Hint Resolve lowerTT_liftTT_switch.
 Hint Rewrite lowerTT_liftTT_switch.
-
 
