devel/Iron/Language/SystemF2Effect/Type.v
@@ -7,4 +7,5 @@ Require Export Iron.Language.SystemF2Effect.Type.Ty.
 Require Export Iron.Language.SystemF2Effect.Type.TyCon.
 Require Export Iron.Language.SystemF2Effect.Type.TyEnv.
 Require Export Iron.Language.SystemF2Effect.Type.Wf.
+Require Export Iron.Language.SystemF2Effect.Type.Mask.
 
