devel/Iron/Language/SystemF2Effect/Type/Mask.v
@@ -1,0 +1,121 @@
+
+Require Import Iron.Language.SystemF2Effect.Type.Ty.
+Require Import Iron.Language.SystemF2Effect.Type.Lift.
+
+
+Fixpoint liftTT_var (n : nat) (d : nat) (ix : nat)
+ := if le_gt_dec d ix
+     then ix + n
+     else ix.
+
+
+(* Mask effects on the given region, 
+   replacing with the bottom effect. *)   (** TODO: let it take the region TCap as well *)
+Fixpoint mask (r : nat) (e : ty) : ty
+ := match e with
+    |  TVar tc       => TVar tc
+    |  TForall k t1  => TForall k (mask (liftTT_var 1 0 r) t1)
+    |  TApp t1 t2    => TApp (mask r t1) (mask r t2)
+    |  TSum t1 t2    => TSum (mask r t1) (mask r t2)
+    |  TBot k        => TBot k
+
+    |  TCon0 tc      => TCon0 tc
+
+    |  TCon1 tc t1
+    => match t1 with
+       | TVar n' 
+       => if beq_nat r n' 
+             then TBot KEffect 
+             else TCon1 tc (mask r t1)
+
+       | _ =>     TCon1 tc (mask r t1)
+       end
+    
+    | TCon2 tc t1 t2 => TCon2 tc (mask r t1) (mask r t2)
+
+    | TCap  tc      => TCap tc
+    end.
+Arguments mask r e : simpl nomatch.
+
+
+Lemma liftTT_mask
+ :  forall r d t
+ ,  mask r (liftTT 1 (r + d) t) = liftTT 1 (r + d) (mask r t).
+Proof.
+ intros. gen r d.
+ induction t; intros; 
+   try (solve [simpl; burn]);
+   try (solve [simpl; f_equal; rewritess; auto]).
+
+ Case "TVar".
+  simpl. lift_cases. simpl. auto.
+  simpl. auto.
+
+  admit.
+
+
+ Case "TCon1".
+  admit. 
+(*
+ simpl.
+  destruct t0.
+
+  SCase "TVar".
+   simpl.
+    lift_cases.
+     unfold mask.
+      break (beq_nat r (n + 1)).
+      break (beq_nat r n).
+       simpl. auto.
+       simpl. lift_cases. norm. 
+ 
+      remember (beq_nat r (n0 + n)) as X. destruct X.
+      remember (beq_nat r n0) as Y. destruct Y.
+       simpl. auto.
+       simpl. lift_cases.
+     
+    
+
+     assert ( mask r (TCon1 TyConRead (TVar (n0 + n)))
+            = if beq_nat r (n0 + n) then TBot KEffect else TCon1 TyConRead (TVar (n0 + n))).
+     simpl.
+     simpl.
+
+     simpl match.
+
+  SCase "TForall".
+    simpl liftTT.
+    set  (X0 := TForall k (liftTT n (S d) t0)).
+     rrwrite (mask r (TCon1 t X0)          = TCon1 t (mask r X0)).
+    subst X0.
+    rrwrite (TForall k (liftTT n (S d) t0) = liftTT n d (TForall k t0)).
+    rewritess. simpl. auto.
+
+  SCase "TApp".
+   simpl liftTT.
+   set      (X0 := TApp (liftTT n d t0_1) (liftTT n d t0_2)).
+    rrwrite (mask r (TCon1 t X0)           = TCon1 t (mask r X0)).
+   subst X0.
+   rrwrite  ( TApp (liftTT n d t0_1) (liftTT n d t0_2)
+            = liftTT n d (TApp t0_1 t0_2)).
+   rewritess. simpl. auto.
+*)
+Qed.
+
+
+Lemma mask_liftTT_id
+ : forall d t
+ , mask d (liftTT 1 d t) = liftTT 1 d t.
+Proof.
+ intros. gen d. 
+ induction t; intros;
+  try (solve [simpl; burn]);
+  try (solve [simpl; f_equal; norm; rewritess; auto]).
+
+ Case "TVar".
+  simpl. lift_cases; burn.
+
+ Case "TCon1".
+   admit.
+Qed.
+
